Foundation/Modal/Kripke/Logic/SobK3.lean
@@ -1,0 +1,105 @@
+import Foundation.Modal.Kripke.Logic.SobK2
+import Foundation.Modal.Kripke.Logic.S4Point3
+
+namespace LO.Modal
+
+open Kripke
+open Hilbert.Kripke
+open GeachConfluent
+
+abbrev Kripke.FrameClass.preorder_connected_mckinsey : FrameClass := { F | IsPreorder _ F ∧ IsConnected _ F ∧ SatisfiesMcKinseyCondition _ F }
+
+namespace Hilbert.SobK3.Kripke
+
+instance sound : Sound (Hilbert.SobK3) Kripke.FrameClass.preorder_connected_mckinsey := instSound_of_validates_axioms $ by
+  apply FrameClass.Validates.withAxiomK;
+  rintro F ⟨_, _, _⟩ _ (rfl | rfl | rfl | rfl);
+  . exact validate_AxiomT_of_reflexive;
+  . exact validate_AxiomFour_of_transitive;
+  . exact validate_axiomM_of_satisfiesMcKinseyCondition;
+  . exact validate_AxiomPoint3_of_connected;
+
+instance consistent : Entailment.Consistent (Hilbert.SobK3) :=
+  consistent_of_sound_frameclass FrameClass.preorder_connected_mckinsey $ by
+    use whitepoint;
+    refine ⟨inferInstance, inferInstance, inferInstance⟩;
+
+instance canonical : Canonical (Hilbert.SobK3) Kripke.FrameClass.preorder_connected_mckinsey := ⟨by
+  apply Set.mem_setOf_eq.mpr;
+  refine ⟨?_, ?_, ?_⟩;
+  . constructor;
+  . infer_instance;
+  . infer_instance;
+⟩
+
+instance complete : Complete (Hilbert.SobK3) Kripke.FrameClass.preorder_connected_mckinsey := inferInstance
+
+end Hilbert.SobK3.Kripke
+
+namespace Logic
+
+open Formula
+open Entailment
+open Kripke
+
+lemma SobK3.Kripke.preorder_connected_mckinsey : Logic.SobK3 = FrameClass.preorder_connected_mckinsey.logic := eq_hilbert_logic_frameClass_logic
+
+@[simp]
+theorem SobK3.proper_extension_of_SobK2 : Logic.SobK2 ⊂ Logic.SobK3 := by
+  constructor;
+  . rw [SobK2.Kripke.preorder_confluent_mckinsey, SobK3.Kripke.preorder_connected_mckinsey]
+    rintro φ hφ F ⟨_, _, _⟩;
+    apply hφ;
+    refine ⟨inferInstance, inferInstance, inferInstance⟩;
+  . suffices ∃ φ, Hilbert.SobK3 ⊢! φ ∧ ¬Kripke.FrameClass.preorder_confluent_mckinsey ⊧ φ by
+      rw [SobK2.Kripke.preorder_confluent_mckinsey];
+      tauto;
+    use (Axioms.Point3 (.atom 0) (.atom 1));
+    constructor;
+    . simp;
+    . apply Kripke.not_validOnFrameClass_of_exists_model_world;
+      let M : Model := ⟨
+        ⟨Fin 4, λ x y => x = 0 ∨ y = 3 ∨ x = y⟩,
+        λ w a => match a with | 0 => w = 1 ∨ w = 3 | 1 => w = 2 ∨ w = 3 | _ => False
+      ⟩;
+      use M, 0;
+      constructor
+      . refine ⟨?_, ⟨?_⟩, ⟨?_⟩⟩;
+        . apply isPreorder_iff _ _ |>.mpr;
+          refine ⟨⟨?_⟩, ⟨?_⟩⟩ <;> omega;
+        . intro x y z ⟨Rxy, Ryz⟩; use 3; simp [M];
+        . intro x; use 3; simp [M];
+      . suffices
+          (∃ x, (0 : M) ≺ x ∧ (∀ (w : M), x ≺ w → w = 1 ∨ w = 3) ∧ x ≠ 2 ∧ x ≠ 3) ∧
+          (∃ x, (0 : M) ≺ x ∧ (∀ (w : M), x ≺ w → w = 2 ∨ w = 3) ∧ x ≠ 1 ∧ x ≠ 3) by
+          simp [M, Semantics.Realize, Satisfies];
+          tauto;
+        constructor;
+        . use 1; simp only [M]; refine ⟨?_, ?_, ?_, ?_⟩ <;> omega;
+        . use 2; simp only [M]; refine ⟨?_, ?_, ?_, ?_⟩ <;> omega;
+
+@[simp]
+theorem SobK3.proper_extension_of_S4Point3 : Logic.S4Point3 ⊂ Logic.SobK3 := by
+  constructor;
+  . exact Hilbert.weakerThan_of_dominate_axioms (by simp) |>.subset;
+  . suffices ∃ φ, Hilbert.SobK3 ⊢! φ ∧ ¬FrameClass.connected_preorder ⊧ φ by
+      rw [S4Point3.Kripke.connected_preorder];
+      tauto;
+    use (Axioms.M (.atom 0))
+    constructor;
+    . simp;
+    . apply Kripke.not_validOnFrameClass_of_exists_model_world;
+      let M : Model := ⟨⟨Fin 2, λ x y => True⟩, λ w _ => w = 0⟩;
+      use M, 0;
+      constructor;
+      . refine ⟨?_, ⟨?_⟩⟩;
+        . apply isPreorder_iff _ _ |>.mpr;
+          refine ⟨⟨?_⟩, ⟨?_⟩⟩ <;> tauto;
+        . tauto;
+      . suffices ∃ x : M, x ≠ 0 by simpa [M, Semantics.Realize, Satisfies];
+        use 1;
+        trivial;
+
+end Logic
+
+end LO.Modal
